compiles

HumanEvalLean/HumanEval40.lean
@@ -1,7 +1,109 @@
 module
 
-def triples_sum_to_zero : Unit :=
-  ()
+public import Std
+import all Init.Data.Range.Polymorphic.UpwardEnumerable
+open Std Std.Do
+
+public def triplesSumToZero (xs : Array Int) : Bool := Id.run do
+  let mut index : Std.TreeSet Int := ∅
+  for h : i in 1...xs.size do
+    -- ensures index ~ xs.take (i - 1)
+    -- ensures: no triple with i₂ < i
+    index := index.insert xs[i - 1]
+    -- ensures index ~ xs.take i
+    for h' : j in i<...xs.size do
+      -- ensures index ~ xs.take i
+      -- ensures: no triple with i₂ < i ∨ i₂ = i ∧ i₃ < j
+      if -(xs[i] + xs[j]) ∈ index then
+        return true
+      -- ensures: no triple with i₂ < i ∨ i₂ = i ∧ i₃ ≤ j
+    -- ensures index ~ xs.take i
+    -- ensures: no triple with i₂ ≤ i
+  return false
+
+def HasTriple (xs : List Int) : Prop :=
+  ∃ (i j k : Nat) (hi : i < j) (hj : j < k) (hk : k < xs.length), xs[i] + xs[j] + xs[k] = 0
+
+def HasTriple₁ (xs : List Int) (m : Nat) : Prop :=
+  ∃ (i j k : Nat) (hi : i < j) (hj : j < k) (hk : k < xs.length)
+    (h : j < m), xs[i] + xs[j] + xs[k] = 0
+
+def HasTriple₂ (xs : List Int) (m n : Nat) : Prop :=
+  ∃ (i j k : Nat) (hi : i < j) (hj : j < k) (hk : k < xs.length)
+    (h : j < m ∨ j = m ∧ k < n), xs[i] + xs[j] + xs[k] = 0
+
+theorem Nat.eq_add_of_toList_rco_eq_append_cons {a b : Nat} {pref cur suff}
+    (h : (a...b).toList = pref ++ cur :: suff) :
+    cur = a + pref.length := by
+  have := Rco.eq_succMany?_of_toList_eq_append_cons h
+  simpa [Std.PRange.UpwardEnumerable.least, PRange.least?] using this
+
+theorem Nat.eq_add_of_toList_roo_eq_append_cons {a b : Nat} {pref cur suff}
+    (h : (a<...b).toList = pref ++ cur :: suff) :
+    cur = a + 1 + pref.length := by
+  apply eq_add_of_toList_rco_eq_append_cons h
+
+theorem Nat.eq_add_of_toList_rio_eq_append_cons {a : Nat} {pref cur suff}
+    (h : (*...a).toList = pref ++ cur :: suff) :
+    cur = pref.length := by
+  have := Rio.eq_succMany?_of_toList_eq_append_cons h
+  simpa [PRange.UpwardEnumerable.least, PRange.least?] using this
+
+attribute [grind =] Nat.length_toList_rco Nat.length_toList_roo
+
+theorem bla :
+    HasTriple₁ xs (i + 1) ↔ HasTriple₂ xs i xs.length := by
+  grind [HasTriple₁, HasTriple₂]
+
+theorem triplesSumToZero_iff {xs : Array Int} :
+    triplesSumToZero xs ↔ HasTriple xs.toList := by
+  generalize hwp : triplesSumToZero xs = wp
+  apply Id.of_wp_run_eq hwp
+  mvcgen
+  invariants
+  · .withEarlyReturn
+      (fun cur index => ⌜(∀ x, x ∈ index ↔ x ∈ xs.take cur.pos) ∧ ¬ HasTriple₁ xs.toList (1 + cur.pos)⌝)
+      (fun ret index => ⌜ret = HasTriple xs.toList⌝)
+  · by
+      rename_i a i c d e f g
+      exact .withEarlyReturn
+        (fun cur index => ⌜¬ HasTriple₂ xs.toList (i) (i + 1 + cur.pos)⌝)
+        (fun ret _ => ⌜ret = HasTriple xs.toList⌝)
+  case vc1 pref cur suff heq _ _ h_mem_iff pref' cur' suff' heq' _ h_mem _ =>
+    have := Nat.eq_add_of_toList_rco_eq_append_cons heq
+    have := Nat.eq_add_of_toList_roo_eq_append_cons heq'
+    simp_all
+    simp +zetaDelta only [h_mem_iff, Array.mem_extract_iff_getElem,
+      TreeSet.mem_insert] at h_mem
+    rcases h_mem with h_mem | h_mem
+    · exact ⟨cur - 1, 1 + pref.length, 1 + pref.length + 1 + pref'.length, by grind⟩
+    · obtain ⟨k, hk, hk'⟩ := h_mem
+      exact ⟨k, 1 + pref.length, 1 + pref.length + 1 + pref'.length, by grind⟩
+  case vc2 pref cur suff heq _ _ h_mem_iff pref' cur' suff' heq' _ h_mem _ =>
+    have := Nat.eq_add_of_toList_rco_eq_append_cons heq
+    have := Nat.eq_add_of_toList_roo_eq_append_cons heq'
+    simp_all
+    simp +zetaDelta [h_mem_iff] at h_mem
+    grind [Array.mem_extract_iff_getElem, HasTriple₂]
+  case vc3 pref cur suff heq _ _ _ =>
+    have := Nat.eq_add_of_toList_rco_eq_append_cons heq
+    grind [HasTriple, HasTriple₁, HasTriple₂]
+  case vc4 pref cur suff heq _ _ h_mem_iff _ _ _ =>
+    have := Nat.eq_add_of_toList_rco_eq_append_cons heq
+    simp only [Array.mem_extract_iff_getElem] at *
+    simp only [reduceCtorEq, false_and, and_false, exists_const, or_false] at h_mem_iff
+    simp +zetaDelta only [TreeSet.mem_insert, h_mem_iff,
+      Nat.zero_add, List.Cursor.pos_mk, List.length_append, List.length_cons, List.length_nil]
+    simp only [LawfulEqCmp.compare_eq_iff_eq, Nat.sub_zero, true_and,
+      reduceCtorEq, eq_iff_iff, false_and, exists_const, or_false]
+    grind [HasTriple, HasTriple₁, HasTriple₂, compare_eq_eq]
+  case vc5 =>
+    grind [HasTriple, HasTriple₁, HasTriple₂]
+  case vc6 =>
+    grind [HasTriple, HasTriple₁, HasTriple₂]
+  case vc7 =>
+    grind [HasTriple, HasTriple₁, HasTriple₂]
+  case vc8 => grind
 
 /-!
 ## Prompt
